src/promising/TsoPtoPF.v
@@ -51,6 +51,7 @@ Proof.
                          lc0.(Local.vwn)
                          lc0.(Local.vro)
                          lc0.(Local.vwo)
+                         lc0.(Local.fwdbank)
                          (Promises.set (S (length mem1)) lc0.(Local.promises))).
         inv LOCAL0.
         { econs 1; eauto. }
